theories/SLOT/EventTrace.v
@@ -1,29 +1,33 @@
 From Coq Require Import
      List.
 
-Reserved Notation "pid '@' req '<~' ret" (at level 30).
+Class EvtContext {PID Req : Set} {Ret : Req -> Set} : Type :=
+  mkCtx { }.
+(* Record Ctx : Type := *)
+(*   mkCtx { ctx_pid_t : Set; *)
+(*           ctx_req_t : Set; *)
+(*           ctx_ret_t : ctx_req_t -> Set; *)
+(*         }. *)
 
-Record Ctx : Type :=
-  mkCtx { ctx_pid_t : Set;
-          ctx_req_t : Set;
-          ctx_ret_t : ctx_req_t -> Set;
-        }.
+Section defs.
+  Context `{EvtContext}.
 
-Record TraceElem {ctx : Ctx} : Set :=
-  trace_elem { te_pid : ctx_pid_t ctx;
-               te_req : ctx_req_t ctx;
-               te_ret : (ctx_ret_t ctx) te_req;
-             }.
+  Record TraceElem : Set :=
+    trace_elem { te_pid : PID;
+                 te_req : Req;
+                 te_ret : Ret te_req;
+               }.
 
-Definition Trace {ctx : Ctx} := list (@TraceElem ctx).
+  Definition Trace := list TraceElem.
+End defs.
 
-Notation "pid '@' ret '<~' req" := (trace_elem _ pid req ret).
+Global Notation "pid '@' ret '<~' req" := (trace_elem pid req ret)(at level 30).
 
 (* Require Import ssreflect ssrfun. *)
 
-Section props.
-  Context {ctx : Ctx}.
-  Let ret_t := ctx_ret_t ctx.
+(* Section props. *)
+(*   Context {ctx : Ctx}. *)
+(*   Let ret_t := ctx_ret_t ctx. *)
 
   (* Lemma te_ret_dual_elim pid (P : forall req, ret_t req -> Prop) req1 (ret1 : ret_t req1) req2 (ret2 : ret_t req2) : *)
   (*     trace_elem ctx pid req1 ret1 = trace_elem ctx pid req2 ret2 -> *)
@@ -39,4 +43,4 @@ Section props.
   (*     trace_elem ctx pid req ret1 = trace_elem ctx pid req ret2 -> *)
   (*     ret1 = ret2. *)
   (* Admitted. *)
-End props.
+(* End props. *)
